Verified interpreter halfway done

theories/Map.v
@@ -43,10 +43,29 @@ Proof.
   split. { intro F. apply N in F as []. } intro D. discriminate D.
 Qed.
 
+Lemma find_dec {T} (m : to T) k
+  : {exists v, Find m k v} + {forall v, ~Find m k v}.
+Proof.
+  destruct (find m k) as [v |] eqn:F; [left | right].
+  - exists v. apply find_iff. exact F.
+  - intros v C. apply find_iff in C. rewrite F in C. discriminate C.
+Qed.
+
+Variant found {T} (m : to T) k : Type :=
+  | Found (v : T) (Y : Find m k v)
+  | NotFound (N : forall v, ~Find m k v)
+  .
+
+Lemma found_dec {T} (m : to T) k : found m k. Proof.
+  destruct (find m k) as [v |] eqn:F; [eleft | right]. { apply find_iff. exact F. }
+  intros v C. apply find_iff in C. rewrite F in C. discriminate C.
+Defined.
+
 
 
 Definition ForAll {T} (P : Name.name -> T -> Prop) (m : to T) : Prop :=
   forall k v (F : Find m k v), P k v.
+Arguments ForAll {T} P m/.
 
 Definition for_all : forall T, (Name.name -> T -> bool) -> to T -> bool := @MapCore.for_all.
 Arguments for_all {T} p m : rename, simpl never.
@@ -459,6 +478,13 @@ Proof.
     split. { intro F. split. { symmetry. exact N. } exact F. } intros [_ F]. exact F.
 Qed.
 
+Lemma remove_if_present_eq {T k1} {m1 m1' : to T} (R1 : RemoveIfPresent k1 m1 m1')
+  {k2} (Ek : k1 = k2)
+  {m2} (Em : Map.Eq m1 m2)
+  {m2'} (Em' : Map.Eq m1' m2')
+  : RemoveIfPresent k2 m2 m2'.
+Proof. subst. cbn in *. intros x y. rewrite <- Em'. rewrite R1. rewrite Em. reflexivity. Qed.
+
 Lemma remove_if_present_det {T k1} {m1 m1' : to T} (R1 : RemoveIfPresent k1 m1 m1')
   {k2} (Ek : k1 = k2)
   {m2} (Em : Map.Eq m1 m2)
@@ -669,10 +695,10 @@ Arguments minus {T} everything discard/.
 Lemma minus_minus {T} (everything : to T) discard
   : Minus everything discard (minus everything discard).
 Proof.
-  cbn. intros. unfold fold. rewrite MapCore.fold_spec. assert (Iff :
-    (Find everything k v /\ (forall (discarded : exists v, Find discard k v), False)) <->
-    (Find everything k v /\ (forall (discarded : exists v,
-      SetoidList.InA MapCore.eq_key_elt (k, v) (MapCore.bindings discard)), False))). {
+  cbn. intros. unfold fold. rewrite MapCore.fold_spec. assert (Iff
+    : (Find everything k v /\ (forall (discarded : exists v, Find discard k v), False)) <->
+      (Find everything k v /\ (forall (discarded : exists v,
+        SetoidList.InA MapCore.eq_key_elt (k, v) (MapCore.bindings discard)), False))). {
     split; intros [F N]; (split; [exact F |]); intros [v' N'];
     apply N; exists v'; apply MapCore.bindings_spec1; exact N'. } rewrite Iff; clear Iff.
   remember (MapCore.bindings discard) as b eqn:Eb; clear discard Eb; rename b into discard.
@@ -793,6 +819,7 @@ Proof.
     destruct l. { invert H1. } constructor. eapply Name.trans. { eassumption. } invert H. assumption.
 Qed.
 
+(*
 Lemma bindings_eq {T} a b
   : @Eq T a b <-> MapCore.bindings a = MapCore.bindings b.
 Proof.
@@ -835,4 +862,251 @@ Proof.
       unfold MapCore.lt_key in L. cbn in L. unfold Name.lt in H.
       rewrite Name.antisym in L. rewrite H in L. discriminate L.
   - intros x y. unfold Find. repeat rewrite <- MapCore.bindings_spec1. rewrite E. reflexivity.
+Qed.
+*)
+
+Lemma eq_key_elt {T} k (v : T) li
+  : SetoidList.InA MapCore.eq_key (k, v) li <-> exists v, SetoidList.InA MapCore.eq_key_elt (k, v) li.
+Proof.
+  induction li as [| [k' v'] tail IH]; cbn in *; (split; [intro I | intros [v'' I]]); invert I.
+  - unfold MapCore.eq_key in H0. cbn in H0. subst. eexists. left. split; reflexivity.
+  - apply IH in H0 as [v'' I]. eexists. right. exact I.
+  - destruct H0; cbn in *; subst. left. reflexivity.
+  - right. apply IH. eexists. exact H0.
+Qed.
+
+Lemma sorted_eq {T} (a b : list (_ * T))
+  (Sa : Sorted.Sorted MapCore.lt_key a) (NDa : SetoidList.NoDupA MapCore.eq_key a)
+  (Sb : Sorted.Sorted MapCore.lt_key b) (NDb : SetoidList.NoDupA MapCore.eq_key b)
+  : (a = b) <-> (forall kv, SetoidList.InA MapCore.eq_key_elt kv a <-> SetoidList.InA MapCore.eq_key_elt kv b).
+Proof.
+  split; intro E. { rewrite E. reflexivity. }
+  generalize dependent b. generalize dependent NDa. induction Sa as [| [ka va] a' Sa' IH La']; intros; cbn in *. {
+    destruct b. { reflexivity. } eassert (I : SetoidList.InA MapCore.eq_key_elt p (p :: b)). {
+      left. split; reflexivity. } apply E in I. invert I. }
+  invert NDa as [| ? ? Na' NDa']. specialize (IH NDa'). invert NDb as [| [kb vb] b' Nb' NDb']. {
+    eassert (I : SetoidList.InA MapCore.eq_key_elt (ka, va) ((ka, va) :: a')). {
+      left. split; reflexivity. } apply E in I. invert I. }
+  invert Sb as [| ? ? Sb' Lb']. specialize (IH _ Sb' NDb'). destruct (Name.compare_spec ka kb) as [Ek | Lk | Gk].
+  - cbn in Ek. subst. rename kb into k. assert (I : SetoidList.InA MapCore.eq_key_elt
+      (k, va) ((k, va) :: a')). { left. split; reflexivity. }
+    apply E in I. invert I. 2: { contradiction Nb'. apply eq_key_elt. eexists. eassumption. }
+    destruct H0 as [_ Ev]; cbn in *; subst. f_equal. apply IH. intros [k' v'].
+    destruct (Name.spec k' k). { subst. split; intro I; [contradiction Na' | contradiction Nb'];
+      apply eq_key_elt; eexists; exact I. }
+    split; intro I; eapply SetoidList.InA_cons_tl in I; apply E in I; (invert I; [| assumption]);
+    destruct H0; cbn in *; subst; contradiction N; reflexivity.
+  - assert (A : SetoidList.InA MapCore.eq_key_elt (ka, va) ((kb, vb) :: b')). { apply E. left. split; reflexivity. }
+    invert A. { destruct H0; cbn in *; subst. rewrite Name.compare_refl in Lk. discriminate Lk. }
+    assert (L : MapCore.lt_key (kb, vb) (ka, va)). { eapply sorted_lt; try exact H0; eassumption. }
+    unfold MapCore.lt_key in L. cbn in L. unfold Name.lt in Lk.
+    rewrite Name.antisym in L. rewrite Lk in L. discriminate L.
+  - assert (A : SetoidList.InA MapCore.eq_key_elt (kb, vb) ((ka, va) :: a')). { apply E. left. split; reflexivity. }
+    invert A. { destruct H0; cbn in *; subst. rewrite Name.compare_refl in Gk. discriminate Gk. }
+    assert (L : MapCore.lt_key (ka, va) (kb, vb)). { eapply sorted_lt; try exact H0; eassumption. }
+    unfold MapCore.lt_key in L. cbn in L. unfold Name.lt in Gk.
+    rewrite Name.antisym in L. rewrite Gk in L. discriminate L.
+Qed.
+
+Lemma bindings_eq {T} a b
+  : @Eq T a b <-> MapCore.bindings a = MapCore.bindings b.
+Proof.
+  cbn. rewrite sorted_eq; try apply MapCore.bindings_spec2; try apply MapCore.bindings_spec2w.
+  unfold Find. split; [intros E [k v] | intros E k v];
+  [repeat rewrite MapCore.bindings_spec1 | repeat rewrite <- MapCore.bindings_spec1]; apply E.
+Qed.
+
+
+
+(*Lemma hd_rel_filter {T} k (v : T) tail (HR : Sorted.HdRel MapCore.lt_key (k, v) tail) (S : Sorted.Sorted MapCore.lt_key (k, v) tail) f*)
+(*  : Sorted.HdRel MapCore.lt_key (k, v) (List.filter f tail).*)
+(*Proof.*)
+(*  generalize dependent v. generalize dependent k.*)
+(*  induction tail as [| [k v] tail IH]; intros; cbn in *. { constructor. }*)
+(*  invert S. unfold MapCore.lt_key in H0; cbn in *. destruct (f (k, v)) eqn:E. { constructor. assumption. }*)
+(*  - constructor.*)
+(*Qed.*)
+
+Lemma in_a_filter {T} {li : list T} {P f x} (I : SetoidList.InA P x (List.filter f li))
+  : SetoidList.InA P x li.
+Proof.
+  generalize dependent I. induction li as [| head tail IH]; intros; cbn in *. { invert I. }
+  destruct (f head) eqn:F. 2: { right. apply IH. exact I. }
+  invert I; [left | right]. { assumption. } apply IH. assumption.
+Qed.
+
+Lemma sorted_filter {T} (li : list (_ * T)) (S : Sorted.Sorted MapCore.lt_key li)
+  (ND : SetoidList.NoDupA MapCore.eq_key li) f
+  : Sorted.Sorted MapCore.lt_key (List.filter f li).
+Proof.
+  induction S as [| [k v] tail S IH L]; intros; cbn in *. { constructor. }
+  invert ND. specialize (IH H2). destruct (f (k, v)) eqn:E. 2: { exact IH. } constructor. { exact IH. }
+  destruct (List.filter f tail) as [| [k' v'] tail'] eqn:F. { constructor. }
+  invert IH. constructor. eapply sorted_lt; [| | eassumption | |]; try eassumption.
+  eapply in_a_filter. rewrite F. left. split; reflexivity.
+Qed.
+
+Lemma no_dup_filter {T} (li : list (_ * T)) (ND : SetoidList.NoDupA MapCore.eq_key li) f
+  : SetoidList.NoDupA MapCore.eq_key (List.filter f li).
+Proof.
+  induction ND as [| [k v] tail N ND IH]; cbn in *. { constructor. }
+  destruct (f (k, v)) eqn:F. 2: { exact IH. } constructor. 2: { exact IH. }
+  intro C. apply N. eapply in_a_filter. exact C.
+Qed.
+
+Lemma bindings_remove {T} x (m : to T)
+  : MapCore.bindings (remove x m) = List.filter (fun kv => negb (Name.eqb x (fst kv))) (MapCore.bindings m).
+Proof.
+  apply sorted_eq. { apply MapCore.bindings_spec2. } { apply MapCore.bindings_spec2w. } {
+    apply sorted_filter. { apply MapCore.bindings_spec2. } apply MapCore.bindings_spec2w. } {
+    apply no_dup_filter. apply MapCore.bindings_spec2w. }
+  intros [k v]. repeat rewrite MapCore.bindings_spec1.
+  unfold remove. rewrite <- MapCore.find_spec. destruct (Name.spec k x).
+  - subst. rewrite MapCore.remove_spec1. split. { intro D. discriminate D. }
+    intro I. remember (MapCore.bindings m) as b eqn:Eb; clear m Eb.
+    induction b as [| [k' v'] tail IH]; cbn in *. { invert I. }
+    destruct (Name.spec x k'); subst; cbn in *. { apply IH. exact I. } invert I. 2: { apply IH. assumption. }
+    destruct H0; cbn in *; subst. contradiction N. reflexivity.
+  - rewrite MapCore.remove_spec2. 2: { intros ->. contradiction N. reflexivity. }
+    rewrite MapCore.find_spec. rewrite <- MapCore.bindings_spec1.
+    remember (MapCore.bindings m) as b eqn:Eb; clear m Eb.
+    generalize dependent x. induction b as [| [k' v'] tail IH]; intros; cbn in *. { reflexivity. }
+    destruct (Name.spec x k'); subst; cbn in *.
+    + rewrite <- IH. 2: { assumption. } split; intro I. 2: { right. exact I. }
+      invert I. { destruct H0; cbn in *; subst. contradiction N. reflexivity. } assumption.
+    + split; intro I; (invert I; [left; assumption | right]); (eapply IH; [exact N |]); assumption.
+Qed.
+
+
+
+Definition cardinality {T} : to T -> nat := MapCore.cardinal.
+Arguments cardinality {T} m : simpl never.
+
+Lemma cardinality_remove {T} (m : to T) k
+  : cardinality (remove k m) =
+    match find m k with
+    | None => cardinality m
+    | Some _ => Nat.pred (cardinality m)
+    end.
+Proof.
+  unfold cardinality. rewrite MapCore.cardinal_spec. rewrite bindings_remove. destruct (find_spec m k).
+  - rewrite MapCore.cardinal_spec. apply MapCore.bindings_spec1 in Y. assert (ND := MapCore.bindings_spec2w m).
+    remember (MapCore.bindings m) as b eqn:Eb; clear m Eb; rename b into li.
+    induction ND as [| [k' v'] tail N ND IH]; intros; cbn in *. { reflexivity. }
+    destruct (Name.spec k k'); subst; cbn in *. 2: {
+      invert Y. { destruct H0; cbn in *; subst. contradiction N0. reflexivity. } rewrite IH. 2: { assumption. }
+      apply PeanoNat.Nat.succ_pred. intro E. destruct H0; discriminate E. }
+    invert Y. 2: { contradiction N. apply eq_key_elt. eexists. eassumption. }
+    destruct H0 as [_ E]; cbn in *; subst. clear IH.
+    rewrite List.forallb_filter_id. { reflexivity. }
+    generalize dependent v'. generalize dependent k'.
+    induction ND as [| [k v] tail N ND IH]; intros; cbn in *. { reflexivity. }
+    destruct (Name.spec k' k); cbn in *. { subst. contradiction N0. left. reflexivity. }
+    eapply IH. intro C. apply N0. right. exact C.
+  - rewrite List.forallb_filter_id. { symmetry. apply MapCore.cardinal_spec. }
+    destruct List.forallb eqn:F. { reflexivity. } assert (A : exists v, Find m k v). 2: {
+      destruct A as [k' F']. apply N in F' as []. } clear N.
+    assert (A : (exists v, Find m k v) <-> exists v, SetoidList.InA MapCore.eq_key_elt (k, v) (MapCore.bindings m)). {
+      split; intros [v F']; exists v; apply MapCore.bindings_spec1; exact F'. } apply A; clear A.
+    remember (MapCore.bindings m) as b eqn:Eb; clear m Eb; rename b into li.
+    induction li as [| [k' v'] tail IH]; intros; cbn in *. { discriminate F. }
+    destruct (Name.spec k k'); subst; cbn in *. { eexists. left. split; reflexivity. }
+    specialize (IH F) as [v IH]. exists v. right. exact IH.
+Qed.
+
+
+
+Definition Pop {T} m k (v : T) leftover : Prop :=
+  Find m k v /\ RemoveIfPresent k m leftover.
+Arguments Pop {T} m k v leftover/.
+
+(* TODO: this could be made much faster if we cracked open the definition of `remove` to do it all in one pass *)
+Definition pop {T} (m : to T) k := option_map (fun v => (v, remove k m)) (find m k).
+Arguments pop {T} m k/.
+
+Lemma pop_eq {T}
+  {m1 : to T} {k1 v1 l1} (P1 : Pop m1 k1 v1 l1)
+  {m2} (Em : Eq m1 m2)
+  {k2} (Ek : k1 = k2)
+  {v2} (Ev : v1 = v2)
+  {l2} (El : Eq l1 l2)
+  : Pop m2 k2 v2 l2.
+Proof.
+  subst. destruct P1 as [F1 R1]. split. { apply Em. exact F1. }
+  eapply remove_if_present_eq; try reflexivity; eassumption.
+Qed.
+
+Lemma pop_det {T}
+  {m1 : to T} {k1 v1 l1} (P1 : Pop m1 k1 v1 l1)
+  {m2} (Em : Eq m1 m2)
+  {k2} (Ek : k1 = k2)
+  {v2 l2} (P2 : Pop m2 k2 v2 l2)
+  : v1 = v2 /\ Eq l1 l2.
+Proof.
+  subst. destruct P1 as [F1 R1]. destruct P2 as [F2 R2]. apply Em in F2. split. { eapply find_det; eassumption. }
+  eapply remove_if_present_det; try reflexivity; eassumption.
+Qed.
+
+Lemma pop_spec {T} (m : to T) k
+  : Reflect.Option (fun pair => Pop m k (fst pair) (snd pair)) (pop m k).
+Proof.
+  unfold Pop. unfold pop. destruct (find_spec m k); simpl option_map; constructor; simpl fst; simpl snd.
+  - split. { exact Y. } apply remove_if_present_remove.
+  - intros [v leftover] [F R]; simpl fst in *; simpl snd in *. apply N in F as [].
+Qed.
+
+
+
+Definition Disjoint {A B} (a : to A) (b : to B) :=
+  forall k (Ma : In a k) (Mb : In b k), False.
+Arguments Disjoint {A B} a b/.
+
+Definition disjoint {A B} (a : to A) : to B -> bool :=
+  for_all (fun k v => negb (in_ a k)).
+Arguments disjoint {A B} a/ b.
+
+Lemma disjoint_spec {A B} (a : to A) (b : to B)
+  : Reflect.Bool (Disjoint a b) (disjoint a b).
+Proof.
+  eapply Reflect.bool_eq. 2: { eapply (@for_all_spec _ (fun k _ => ~In a k)). intros k _.
+    destruct (in_spec a k); constructor. { intro C. apply C. exact Y. } intro C. apply N. exact C. }
+  cbn. split; intros F k.
+  - intros vb Fb [va Fa]. eapply F; eexists; eassumption.
+  - intros [va Fa] [vb Fb]. eapply F. { exact Fb. } eexists. exact Fa.
+Qed.
+
+Lemma in_bindings {T} (m : to T) k
+  : In m k <-> List.In k (List.map fst (MapCore.bindings m)).
+Proof.
+  split.
+  - intros [v F]. apply MapCore.bindings_spec1 in F. remember (MapCore.bindings m) as b eqn:Eb; clear m Eb.
+    generalize dependent v. generalize dependent k. induction b as [| [k v] tail IH]; intros; cbn in *. { invert F. }
+    invert F; [left | right]. { destruct H0; cbn in *; subst. reflexivity. } eapply IH. exact H0.
+  - intro I. assert (Iff : In m k <-> exists v, SetoidList.InA MapCore.eq_key_elt (k, v) (MapCore.bindings m)).
+    + split; intros [v F]; exists v; apply MapCore.bindings_spec1; exact F.
+    + apply Iff. clear Iff. remember (MapCore.bindings m) as b eqn:Eb; clear m Eb. generalize dependent k.
+      induction b as [| [k v] tail IH]; intros; cbn in *. { destruct I. }
+      destruct I as [-> | I]. { eexists. left. split; reflexivity. }
+      specialize (IH _ I) as [v' F]. eexists. right. exact F.
+Qed.
+
+Lemma not_disjoint_exists {A B} {a : to A} {b : to B} (N : forall (D : Disjoint a b), False)
+  : exists k, In a k /\ In b k.
+Proof.
+  assert (Iff : (exists k, In a k /\ In b k) <-> exists k, (
+    List.In k (List.map fst (MapCore.bindings a)) /\
+    List.In k (List.map fst (MapCore.bindings b)))). {
+    split; intros [k I]; exists k; repeat rewrite in_bindings in *; exact I. } apply Iff. clear Iff.
+  assert (Iff : (forall (D : Disjoint a b), False) <-> forall (D : forall k
+    (Ia : List.In k (List.map fst (MapCore.bindings a)))
+    (Ib : List.In k (List.map fst (MapCore.bindings b))), False), False). {
+    split. 2: { intros C D. apply N in D as []. }
+    intros D C. apply D. intros k Ia Ib. apply in_bindings in Ia. apply in_bindings in Ib.
+    eapply C; eassumption. } rewrite Iff in N. clear Iff.
+  remember (MapCore.bindings a) as ba eqn:Ea; clear a Ea.
+  remember (MapCore.bindings b) as bb eqn:Eb; clear b Eb.
+  generalize dependent B. induction ba as [| [k v] tail IH]; intros; cbn in *. { contradiction N. intros k []. }
+  destruct (List.in_dec Name.eq_dec k (List.map fst bb)). { exists k. split. { left. reflexivity. } assumption. }
+  edestruct IH as [K [IHa IHb]]. 2: { exists K. split. { right. exact IHa. } exact IHb. }
+  intro C. apply N. intros k' [-> | I] C'. { apply n in C' as []. } eapply C; eassumption.
 Qed.
