theories/WellFormed.v
@@ -2,6 +2,9 @@ From LinearCore Require
   BoundIn
   Pattern
   .
+From LinearCore Require Import
+  Invert
+  .
 
 
 
@@ -13,6 +16,50 @@ Inductive Strict : Pattern.strict -> Prop :=
   .
 Arguments Strict strict.
 
+Fixpoint strict_acc strict_pattern :=
+  match strict_pattern with
+  | Pattern.Ctr constructor => Some Map.empty
+  | Pattern.App curried argument =>
+      match strict_acc curried with None => None | Some bound_in_curried =>
+        if Map.in_ bound_in_curried argument then None else Some (Map.overriding_add argument tt bound_in_curried)
+      end
+  end.
+
+Lemma strict_acc_bound_in strict_pattern bindings (E : strict_acc strict_pattern = Some bindings)
+  : Map.Reflect (BoundIn.Strict strict_pattern) bindings.
+Proof.
+  generalize dependent bindings. induction strict_pattern; cbn in *; intros. {
+    invert E. split. { intros [y F]. invert F. } intro B. invert B. }
+  destruct (strict_acc strict_pattern) as [bindings' |] eqn:Es. 2: { discriminate E. }
+  destruct (Map.find_spec bindings' argument); invert E. specialize (IHstrict_pattern _ eq_refl x). split.
+  - intros [v F]. apply Map.find_overriding_add in F as [[-> ->] | [Nx M]]; [left | right].
+    apply IHstrict_pattern. eexists. exact M.
+  - intro B. apply Map.in_overriding_add. invert B; [left | right]. { reflexivity. }
+    apply IHstrict_pattern. exact bound_earlier.
+Qed.
+
+Lemma strict_acc_spec strict_pattern
+  : Reflect.Option (fun _ => Strict strict_pattern) (strict_acc strict_pattern).
+Proof.
+  induction strict_pattern; cbn in *. { constructor. constructor. }
+  assert (R := strict_acc_bound_in strict_pattern). destruct IHstrict_pattern as [bindings |]. 2: {
+    constructor. intros bindings S. invert S. apply N in curried_well_formed as []. exact bindings. }
+  specialize (R _ eq_refl). destruct (Map.find_spec bindings argument); constructor.
+  - intros bindings' S. invert S. apply N. apply R. eexists. eassumption.
+  - constructor. { exact Y. } intro B. apply R in B as [y F]. apply N in F as [].
+Qed.
+
+Definition strict strict_pattern :=
+  match strict_acc strict_pattern with Some _ => true | None => false end.
+Arguments strict strict_pattern/.
+
+Lemma strict_spec strict_pattern
+  : Reflect.Bool (Strict strict_pattern) (strict strict_pattern).
+Proof.
+  unfold strict. destruct (strict_acc_spec strict_pattern); constructor. { exact Y. }
+  apply N. exact Map.empty.
+Qed.
+
 
 
 Inductive MoveOrReference : Pattern.move_or_reference -> Prop :=
@@ -23,6 +70,19 @@ Inductive MoveOrReference : Pattern.move_or_reference -> Prop :=
   .
 Arguments MoveOrReference move_or_reference.
 
+Definition move_or_reference pattern :=
+  match pattern with Pattern.Mov strict_pattern | Pattern.Ref strict_pattern =>
+    strict strict_pattern
+  end.
+Arguments move_or_reference pattern/.
+
+Lemma move_or_reference_spec pattern
+  : Reflect.Bool (MoveOrReference pattern) (move_or_reference pattern).
+Proof.
+  unfold move_or_reference. destruct pattern; destruct (strict_spec strict0); constructor;
+  try (constructor; exact Y); intro C; invert C; apply N in strict_well_formed as [].
+Qed.
+
 
 
 Inductive Pattern : Pattern.pattern -> Prop :=
@@ -32,3 +92,17 @@ Inductive Pattern : Pattern.pattern -> Prop :=
       : Pattern (Pattern.Pat move_or_reference)
   .
 Arguments Pattern pattern.
+
+Definition pattern patt :=
+  match patt with
+  | Pattern.Nam _ => true
+  | Pattern.Pat patt => move_or_reference patt
+  end.
+
+Lemma pattern_spec patt
+  : Reflect.Bool (Pattern patt) (pattern patt).
+Proof.
+  unfold pattern. destruct patt. { constructor. constructor. }
+  destruct (move_or_reference_spec move_or_reference0); constructor. { constructor. exact Y. }
+  intro P. apply N. invert P. assumption.
+Qed.
