theories/Extract.v
@@ -1,5 +1,5 @@
 From LinearCore Require
-  SmallStep
+  SmallStepFunction
   .
 
 Set Extraction Optimize.
@@ -11,10 +11,11 @@ Set Extraction Flag 2047.
 
 Extract Inductive bool => "bool" [ "true" "false" ].
 Extract Inductive list => "list" [ "[]" "( :: )" ].
+Extract Inductive option => "option" [ "Some" "None" ] "(fun some none opt -> match opt with None -> none () | Some x -> some x)".
 Extract Inductive prod => "( * )" [ "(, )" ].
 Extract Inductive sigT => "( * )" [ "(, )" ].
 Extract Inductive sumbool => "bool" [ "true" "false" ].
 Extract Inductive unit => "unit" [ "()" ].
 
 Set Extraction Output Directory "ocaml/lib".
-Recursive Extraction Library Map.
+Recursive Extraction Library SmallStepFunction.
