theories/Fuel.v
@@ -1,0 +1,15 @@
+From Coq.extraction Require
+  Extraction
+  .
+
+
+
+Inductive fuel : Set :=
+  | Stop
+  | Continue (pred : fuel)
+  .
+
+
+
+Extract Inductive fuel => "unit" [ "()" "()" ]
+  "(fun _ f () -> f ())".
