theories/Halt.v
@@ -1,0 +1,19 @@
+From Coq.extraction Require
+  Extraction
+  .
+
+
+
+Inductive halt (T : Type) : Type :=
+  | Return (output : T)
+  | Exit
+  | OutOfFuel
+  .
+Arguments Return {T} output.
+Arguments Exit {T}.
+Arguments OutOfFuel {T}.
+
+
+
+Extract Inductive halt => "option" [ "Some" "None" "(assert false; None)" ]
+  "(fun some none _ opt -> match opt with None -> none () | Some x -> some x)".
