theories/NewNames.v
@@ -24,11 +24,12 @@ Arguments in_/ {T} m k.
 Axiom new_name : Map.set -> Name.name -> Name.name.
 Arguments new_name reserved orig_name.
 Extract Constant new_name =>
-  "let rec new_name' reserved name = if in_ name reserved then unbound' (underscored name) reserved else name in new_name'".
+  "fun reserved -> let rec new_name' name = if in_ reserved name then new_name' (underscored name) else name in new_name'".
 
 Axiom not_in_new_name : forall reserved orig_name (I : Map.In reserved (new_name reserved orig_name)), False.
 Arguments not_in_new_name {reserved orig_name} I.
 
+(* Yes, exactly equal, not just equivalent: *)
 Axiom new_name_det : forall r1 r2 (E : Map.Eq r1 r2) orig_name, new_name r1 orig_name = new_name r2 orig_name.
 Arguments new_name_det {r1 r2} E orig_name.
 
@@ -43,12 +44,12 @@ Arguments generate reserved names/.
 
 
 
-Lemma in_generate_acc acc reserved names k :
-  Map.In (generate_acc acc reserved names) k <-> (Map.In names k \/ Map.In acc k).
+Lemma in_generate_acc acc reserved names k
+  : Map.In (generate_acc acc reserved names) k <-> (Map.In names k \/ Map.In acc k).
 Proof.
-  cbn. unfold Map.fold. rewrite MapCore.fold_spec. assert (Iff :
-    ((exists v, Map.Find names k v) \/ (exists v, Map.Find acc k v)) <->
-    ((exists v, SetoidList.InA MapCore.eq_key_elt (k, v) (MapCore.bindings names)) \/ (exists v, Map.Find acc k v))). {
+  cbn. unfold Map.fold. rewrite MapCore.fold_spec. assert (Iff
+    : ((exists v, Map.Find names k v) \/ (exists v, Map.Find acc k v)) <->
+      ((exists v, SetoidList.InA MapCore.eq_key_elt (k, v) (MapCore.bindings names)) \/ (exists v, Map.Find acc k v))). {
     split; (intros [[v F] | [v F]]; [left | right]; exists v; [| exact F]); apply MapCore.bindings_spec1; exact F. }
   rewrite Iff; clear Iff. remember (MapCore.bindings names) as b eqn:Eb; clear names Eb; rename b into names.
   generalize dependent k. generalize dependent reserved. generalize dependent acc.
@@ -63,6 +64,13 @@ Proof.
     destruct H0; cbn in *; subst. right. eexists. apply Map.find_overriding_add. left. split; reflexivity.
   - right. destruct (Name.spec x k); subst; eexists; apply Map.find_overriding_add;
     [left | right]. { split; reflexivity. } split; eassumption.
+Qed.
+
+Lemma in_generate reserved names k
+  : Map.In (generate reserved names) k <-> Map.In names k.
+Proof.
+  unfold generate. rewrite in_generate_acc. split. 2: { intro I. left. exact I. }
+  intros [I | I]. { exact I. } destruct I as [v F]. invert F.
 Qed.
 
 Lemma not_in_generate_acc
@@ -87,25 +95,22 @@ Lemma not_in_generate
   : False.
 Proof. eapply not_in_generate_acc; try eassumption. intros x I [y C]. invert C. Qed.
 
-Lemma generate_acc_det {a1 a2} (Ea : Map.Eq a1 a2) {r1 r2} (Er : Map.Eq r1 r2) {n1 n2} (En : Map.Eq n1 n2)
-  : Map.Eq (generate_acc a1 r1 n1) (generate_acc a2 r2 n2).
+Lemma generate_acc_det {a1 a2} (Ea : a1 = a2) {r1 r2} (Er : Map.Eq r1 r2) {n1 n2} (En : Map.Eq n1 n2)
+  : generate_acc a1 r1 n1 = generate_acc a2 r2 n2.
 Proof.
-  intros x y. unfold generate. unfold generate_acc. unfold Map.fold.
-  repeat rewrite MapCore.fold_spec. apply Map.bindings_eq in En.
+  unfold generate_acc. unfold Map.fold. repeat rewrite MapCore.fold_spec. apply Map.bindings_eq in En.
   remember (MapCore.bindings n1) as b1 eqn:E1; clear n1 E1; rename b1 into n1.
   remember (MapCore.bindings n2) as b2 eqn:E2; clear n2 E2; rename b2 into n2.
-  subst. rename n2 into names. generalize dependent y. generalize dependent x. generalize dependent r2.
-  generalize dependent r1. generalize dependent a2. generalize dependent a1.
-  induction names as [| [k v] tail IH]; intros; cbn in *. { apply Ea. }
-  apply IH. 2: { exact Er. } intros. repeat rewrite Map.find_overriding_add. rewrite Ea.
-  erewrite new_name_det. { reflexivity. } cbn. intros. repeat rewrite Map.find_iff.
-  repeat rewrite Map.find_overriding_union. destruct (Map.find_spec r1 k1).
-  - apply Er in Y. apply Map.find_iff in Y. rewrite Y. reflexivity.
-  - destruct (Map.find_spec r2 k1). { apply Er in Y. apply N in Y as []. }
-    repeat rewrite <- Map.find_iff. fold (Map.domain a1). fold (Map.domain a2).
-    repeat rewrite Map.find_domain. erewrite Map.in_eq. { reflexivity. } assumption.
+  subst. rename n2 into names. generalize dependent r2. generalize dependent r1. generalize dependent a2.
+  induction names as [| [k v] tail IH]; intros; cbn in *. { reflexivity. }
+  erewrite IH; clear IH. 2: { exact Er. } erewrite new_name_det. { reflexivity. }
+  intros k' v'. repeat rewrite Map.find_iff. repeat rewrite Map.find_overriding_union.
+  destruct (Map.find_spec r1 k'). { apply Er in Y. apply Map.find_iff in Y. rewrite Y. reflexivity. }
+  destruct (Map.find_spec r2 k'). { apply Er in Y. apply N in Y as []. }
+  repeat rewrite <- Map.find_iff. fold (Map.domain a2). repeat rewrite Map.find_domain.
+  erewrite Map.in_eq. { reflexivity. } apply Map.eq_refl.
 Qed.
 
 Lemma generate_det {r1 r2} (Er : Map.Eq r1 r2) {n1 n2} (En : Map.Eq n1 n2)
-  : Map.Eq (generate r1 n1) (generate r2 n2).
-Proof. apply generate_acc_det; try assumption. apply Map.eq_refl. Qed.
+  : generate r1 n1 = generate r2 n2.
+Proof. apply generate_acc_det; try assumption. reflexivity. Qed.
